updates

history.fst
@@ -2,27 +2,127 @@ module History
 
 open FStar.List.Tot
 
+module L = FStar.List.Tot
+
 module Vc = Vector_clock
 
 type state = nat
 
-type ntree = | Ntree: v:nat -> children:list ntree -> ntree
-
-type history =
-| History : clock:Vc.t
+type history (n:nat) =
+| History : clock:Vc.t n
           -> state:state
-          -> children:list history
-          -> history
+          -> children:list (history n)
+          -> history n
 
-let rec wellformed (h:history) : Tot bool (decreases %[h]) =
+val wellformed : #n:nat -> h:history n -> Tot bool (decreases %[h])
+val wellformed' : #n:nat -> l:list (history n) -> parent_clock:Vc.t n -> Tot bool (decreases %[l])
+let rec wellformed h =
   let History clock _ ch = h in
-  wellformed' clock ch
-and wellformed' parent_clock children : Tot bool (decreases %[children]) =
+  wellformed' ch clock
+and wellformed' children parent_clock =
   match children with
   | [] -> true
   | x::xs ->
      let clock = History?.clock x in
-     length clock = length parent_clock &&
      Vc.hb parent_clock clock &&
      wellformed x &&
-     wellformed' parent_clock xs
+     wellformed' xs parent_clock
+
+val mem : #n:nat -> clock:Vc.t n -> h:history n -> Tot bool (decreases %[h])
+val mem' : #n:nat -> l:list (history n) -> clock:Vc.t n -> Tot bool (decreases %[l])
+let rec mem clock h = 
+  let History k _ ch = h in
+  clock = k || mem' ch clock
+and mem' l clock = 
+  match l with
+  | [] -> false
+  | x::xs -> mem clock x || mem' xs clock
+
+
+val size : #n:nat -> h:history n -> Tot nat (decreases %[h])
+val size' : #n:nat -> l:list (history n) -> Tot nat (decreases %[l])
+let rec size h =
+  let History _ _ ch = h in
+  1 + size' ch
+and size' l = 
+  match l with
+  | [] -> 0
+  | x::xs -> size x + size' xs
+
+val lemma1: #n: nat -> h:history n{wellformed h} 
+          -> Lemma (ensures (forall c1 c2. mem c1 h /\ mem c2 h ==> length c1 = length c2)) (decreases (size h))
+let rec lemma1 h = 
+  let History c s ch = h in
+  match ch with
+  | [] -> ()
+  | x::xs -> lemma1 (History c s xs); lemma1 x
+
+val lemma2 : #n:nat -> h:history n{wellformed h}
+           -> Lemma (ensures (forall h'. L.mem h' (History?.children h) ==> wellformed h')) (decreases (size h))
+let rec lemma2 (History c s ch) =
+  match ch with
+  | [] -> ()
+  | x::xs -> assert (wellformed x); lemma2 (History c s xs)
+
+val lemma3 : #n:nat -> h:history n{wellformed h}
+          -> Lemma (ensures (forall h'. L.mem h' (History?.children h) ==> Vc.hbeq (History?.clock h) (History?.clock h'))) (decreases (size h))
+let rec lemma3 (History c s ch) =
+  match ch with
+  | [] -> ()
+  | x::xs -> assert (wellformed x); lemma3 (History c s xs); lemma3 x
+
+val lemma4 : #n:nat -> h:history n{wellformed h}
+           -> Lemma (ensures (forall c. mem c h ==> Vc.hbeq (History?.clock h) c))
+let rec lemma4 h =
+  let History c s ch = h in
+  match ch with
+  | [] -> Vc.hbeq_reflexive c
+  | x::xs -> 
+      lemma4 x;
+      assert (forall c. mem c x ==> Vc.hbeq (History?.clock h) c);
+      admit ()
+    
+val lca : #n:nat 
+        -> h:history n{wellformed h}
+        -> a:Vc.t n 
+        -> b:Vc.t n 
+        -> init:Vc.t n{Vc.hbeq init a /\ Vc.hbeq init b}
+        -> Tot (r:Vc.t n{Vc.hbeq r a /\ Vc.hbeq r b}) (decreases %[h])
+val lca' : #n:nat 
+         -> l:list (history n){forall h. L.mem h l ==> wellformed h} 
+         -> a:Vc.t n 
+         -> b:Vc.t n 
+         -> init:Vc.t n{Vc.hbeq init a /\ Vc.hbeq init b}
+         -> Tot (r:Vc.t n{Vc.hbeq r a /\ Vc.hbeq r b}) (decreases %[l])
+let rec lca h a b init =
+  lemma1 h;
+  lemma2 h;
+  let History clock _ ch = h in
+  assert (forall h. L.mem h ch ==> wellformed h);
+  assert (forall h1 h2. L.mem h1 ch /\ L.mem h2 ch ==> length (History?.clock h1) = length (History?.clock h2));
+  if Vc.hbeq init clock && Vc.hbeq clock a && Vc.hbeq clock b
+  then lca' ch a b clock
+  else init
+and lca' l a b init =
+  match l with
+  | [] -> init 
+  | x::xs -> lca' xs a b (lca x a b init)
+
+val lemma4 : #n:nat
+          -> h:history n{wellformed h}
+          -> a:Vc.t n{mem a h}
+          -> b:Vc.t n{mem b h}
+          -> init:Vc.t n{init = History?.clock h}
+          -> Lemma (ensures (Vc.hbeq init a /\ Vc.hbeq init b))
+let lemma4 h a b init =
+  let History clock _ _ = h in
+  assert (clock = init);
+  Vc.hbeq_reflexive 
+  admit ()
+
+val lca2 : #n:nat
+       -> h:history n{wellformed h}
+       -> a:Vc.t n{mem a h}
+       -> b:Vc.t n{mem b h}
+       -> r:Vc.t n{Vc.hbeq r a /\ Vc.hbeq r b}
+let lca2 h a b = lca h a b (History?.clock h)
