vector_clock.fst
@@ -2,7 +2,7 @@ module Vector_clock
 
 open FStar.List.Tot
 
-type t = v:list nat{Cons? v}
+type t (n:nat) = lst:list nat{n > 0 && length lst = n}
 
 type ordering =
 | Happened_before
@@ -26,15 +26,63 @@ let rec compare' v1 v2 r =
         else compare' xs ys Happened_after
     | x::xs, y::ys, Concurrent -> Concurrent
 
-val compare : v1:t -> v2:t{length v2 = length v1} -> ordering
+val compare : #n:nat -> v1:t n -> v2:t n -> ordering
 let compare v1 v2 = compare' v1 v2 Equal
 
-val hb: v1:t -> v2:t{length v1 = length v2} -> bool
+val hb: #n:nat -> v1:t n -> v2:t n -> bool
 let hb a b = compare a b = Happened_before
 
-val hbeq: v1:t -> v2:t{length v1 = length v2} -> bool
+val hbeq: #n:nat -> v1:t n -> v2:t n -> bool
 let hbeq a b =
   match compare a b with
   | Happened_before | Equal -> true
   | _ -> false
-  
+
+val lemma1 : v:list nat -> Lemma (ensures (compare' v v Equal = Equal)) 
+let rec lemma1 v =
+  match v with
+  | [] -> ()
+  | x::xs -> lemma1 xs
+
+val hbeq_reflexive : #n:nat -> v:t n -> Lemma (ensures (hbeq v v))
+let hbeq_reflexive v = lemma1 v
+
+val lemma2 : v1:list nat -> v2:list nat{length v1 = length v2} -> o:ordering{not (o = Equal)}
+           -> Lemma (ensures (not (compare' v1 v2 o = Equal)))
+let rec lemma2 v1 v2 o =
+  match v1, v2, o with
+  | [], [], _ -> ()
+  | _, _, Concurrent -> ()
+  | x::xs, y::ys, Happened_before -> 
+     if x > y then ()
+     else lemma2 xs ys Happened_before
+  | x::xs, y::ys, Happened_after -> 
+     if x < y then ()
+     else lemma2 xs ys Happened_after
+
+val lemma3 : v1:list nat -> v2:list nat{length v1 = length v2} -> o:ordering 
+           -> Lemma (ensures (compare' v1 v2 o = Equal ==> v1 = v2))
+let rec lemma3 v1 v2 o =
+  match v1, v2, o with
+  | [], [], _ -> ()
+  | x::xs, y::ys, Equal -> 
+      if x = y then lemma3 xs ys Equal
+      else if x < y then lemma2 xs ys Happened_before
+      else lemma2 xs ys Happened_after
+  | x::xs, y::ys, Happened_before ->
+      if x > y then ()
+      else lemma2 xs ys Happened_before
+  | x::xs, y::ys, Happened_after ->
+      if x < y then ()
+      else lemma2 xs ys Happened_after
+  | _, _, Concurrent -> ()
+
+val hbeq_transitive : #n:nat -> v1:t n -> v2:t n{hbeq v1 v2} -> v3:t n{hbeq v2 v3} -> Lemma (ensures (hbeq v1 v3))
+let hbeq_transitive v1 v2 v3 =
+  match compare v1 v2 with
+  | Equal -> lemma3 v1 v2 Equal
+  | Happened_before -> 
+     begin match compare v2 v3 with
+     | Equal -> lemma3 v2 v3 Equal
+     | Happened_before -> admit ()
+     end
